LibOrder

src/LibWf.v
@@ -5,83 +5,42 @@
 
 Set Implicit Arguments.
 Require Import LibTactics LibLogic
- LibProd LibSum LibRelation LibNat.
+ LibProd LibSum LibRelation LibNat LibInt.
 
 
 (* ********************************************************************** *)
 (** * Compatibility *)
 
-(** From the Prelude:
+(** Coq's stdlib Prelude defines:
 
  Inductive Acc A (R:A->A->Prop) (x:A) : Prop :=
-   | Acc_intro : (forall y:A, R y x -> Acc y) -> Acc x.
+   | Acc_intro : (forall (y:A), R y x -> Acc y) -> Acc x.
 
- Definition well_founded A (R:A->A->Prop) := forall (x:A), Acc x.
+ Definition well_founded A (R:A->A->Prop) := 
+    forall (x:A), Acc x.
 
 *)
 
-(** We introduce [wf] as a shorter name for [well_founded], both
+(** TLC introduces [wf] as a shorter name for [well_founded], both
     for conciseness and for tactics to specifically recognize 
     this symbol. *)
 
 Definition wf := well_founded.
 
 
-(* ********************************************************************** *)
-(** * Generalities *)
-
-(* ---------------------------------------------------------------------- *)
-(** ** Inclusion and equivalence *)
-
-(** Well-foundedness preserved by inclusion *)
-
-Lemma incl_wf : forall A (R1 R2 : binary A),
-  wf R1 -> 
-  incl R2 R1 -> 
-  wf R2.
-Proof using.
-  introv W1 Inc. intros x.
-  pattern x. apply (well_founded_ind W1). clear x.
-  intros x IH. constructor. intros. apply IH. apply~ Inc.
-Qed.
-
-
 (* ---------------------------------------------------------------------- *)
 (** ** Tactics *)
 
-(** [solve_wf] is a tactic that tries to prove a goal of the
-    form [wf R]. It is implemented using [auto]. *)
-
-Tactic Notation "solve_wf" :=
-  solve [ auto with wf ].
-
-(** [auto with wf] attempts to unfold names of relations. *)
+(** [auto with wf] attempts to unfold the names of 
+    the relations given as argument to [wf]. *)
 
 Hint Extern 1 (wf ?R) => progress (unfold R) : wf.
 
-(** [unfold_wf] and [unfolds_wf] are shorthands for unfolding
-    combinators used in definitions related to well-foundedness. *)
+(** [solve_wf] is a shorthand for solving goals using
+    [auto with wf], aimed to prove goals of the form [wf R]. *)
 
-Ltac unfold_wf_base :=
-  unfold_unproj; unfold_uncurryp; 
-  unfold lexico4, lexico3, lexico2.
-
-Ltac unfolds_wf_base :=
-  unfolds_unproj; unfolds_uncurryp; unfolds_lexico.
-
-Tactic Notation "unfold_wf" :=
-  unfold_wf_base.
-Tactic Notation "unfold_wf" "~" :=
-  unfold_wf; auto_tilde.
-Tactic Notation "unfold_wf" "*" :=
-  unfold_wf; auto_star.
-
-Tactic Notation "unfolds_wf" :=
-  unfolds_wf_base.
-Tactic Notation "unfolds_wf" "~" :=
-  unfolds_wf; auto_tilde.
-Tactic Notation "unfolds_wf" "*" :=
-  unfolds_wf; auto_star.
+Tactic Notation "solve_wf" :=
+  solve [ auto with wf ].
 
 
 
@@ -95,7 +54,7 @@ Tactic Notation "unfolds_wf" "*" :=
     relates [x] to [y] when [f x < f y], at type [nat]. *)
 
 Definition measure A (f:A->nat) : binary A :=
-  fun x1 x2 => f x1 < f x2.
+  fun x1 x2 => (f x1 < f x2)%nat.
 
 
 (* ---------------------------------------------------------------------- *)
@@ -105,7 +64,7 @@ Section Measure.
 Variables (A : Type).
 Implicit Type f : A -> nat.
 
-Lemma measure_wf : forall f, 
+Lemma wf_measure : forall f, 
   wf (measure f).
 Proof using.
   intros f a. gen_eq n: (f a). gen a. pattern n.
@@ -114,34 +73,39 @@ Proof using.
   rewrite <- Eq in H. apply* IH.
 Qed.
 
-Lemma measure_trans : forall (f : A -> nat), 
+Lemma trans_measure : forall (f : A -> nat), 
   trans (measure f).
 Proof using. intros. unfold measure, trans. intros. nat_math. Qed.
 
-(* TODO: Lemma measure_order *)
+(* -- LATER: Lemma order_measure *)
 
 End Measure.
 
-Hint Resolve measure_wf : wf.
+Hint Resolve wf_measure : wf.
 
 
 (* ---------------------------------------------------------------------- *)
 (** ** Measure on pairs *)
 
 Definition measure2 A1 A2 (f : A1 -> A2 -> nat) : binary (A1*A2) :=
-  fun p1 p2 => let (x1,y1) := p1 in let (x2,y2) := p2 in f x1 y1 < f x2 y2.
+  fun p1 p2 => let (x1,y1) := p1 in 
+               let (x2,y2) := p2 in 
+               (f x1 y1 < f x2 y2)%nat.
 
-Lemma measure2_wf : forall A1 A2 (f:A1->A2->nat), wf (measure2 f).
+Lemma wf_measure2 : forall A1 A2 (f:A1->A2->nat), 
+  wf (measure2 f).
 Proof using.
   intros A1 A2 f [x1 x2]. apply (@measure_induction _ (uncurry2 f)). clear x1 x2.
   intros [x1 x2] H. apply Acc_intro. intros [y1 y2] Lt. apply~ H.
 Qed.
 
-Hint Resolve measure2_wf : wf.
+Hint Resolve wf_measure2 : wf.
 
 
 (* ---------------------------------------------------------------------- *)
-(** Extension of [induction_wf] tactic for [measure] *)
+(** Extension of LibTactic's [induction_wf] tactic for [measure] *)
+
+(** -- LATER: introduce a hook in LibTactics to reduce copy-paste *)
 
 Ltac induction_wf_core_then IH E X cont ::=
   let T := type of E in
@@ -151,7 +115,7 @@ Ltac induction_wf_core_then IH E X cont ::=
   match T with
   (* To support for [measure] from LibWf, we add the next two lines: *)
   | ?A -> nat =>
-     induction_wf_core_then IH (measure_wf E) X cont
+     induction_wf_core_then IH (wf_measure E) X cont
   (* End of modification *)
   | ?A -> ?A -> Prop =>
      pattern X;
@@ -172,12 +136,32 @@ Ltac induction_wf_core_then IH E X cont ::=
 
 
 (* ********************************************************************** *)
-(** * Empty relation *)
+(** * Construction of well-founded relations *)
 
-Lemma empty_wf : forall A, wf (@empty A).
+(* ---------------------------------------------------------------------- *)
+(** ** Empty relation *)
+
+Lemma empty_wf : forall A,
+  wf (@empty A).
 Proof using. intros_all. constructor. introv H. false. Qed.
 
 Hint Resolve empty_wf : wf.
+
+
+(* ---------------------------------------------------------------------- *)
+(** ** Inclusion *)
+
+(** Well-foundedness preserved by inclusion *)
+
+Lemma wf_of_rel_incl : forall A (R1 R2 : binary A),
+  wf R1 -> 
+  rel_incl R2 R1 -> 
+  wf R2.
+Proof using.
+  introv W1 Inc. intros x.
+  pattern x. apply (well_founded_ind W1). clear x.
+  intros x IH. constructor. intros. apply IH. apply~ Inc.
+Qed.
 
 
 (* ********************************************************************** *)
@@ -188,7 +172,7 @@ Hint Resolve empty_wf : wf.
 
 (** The relation "less than" on natural numbers is well_founded. *)
 
-Lemma lt_wf : wf lt.
+Lemma lt_wf : wf Peano.lt.
 Proof using.
   intros x.
   induction x using peano_induction. apply~ Acc_intro.
@@ -201,13 +185,18 @@ Hint Resolve lt_wf : wf.
 (** ** The relation "greater than" on the set of
        natural number lower than a fixed upper bound. *)
 
-Definition nat_upto (b : nat) :=
-  fun n m : nat => (n <= b) /\ (m < n)%nat.
+Definition nat_upto (b:nat) :=
+  fun (n m:nat) => (n <= b)%nat /\ (m < n)%nat.
 
-Lemma nat_upto_wf : forall b, wf (nat_upto b).
+Lemma nat_upto_eq : forall (b n m:nat),
+  nat_upto b n m = ((n <= b)%nat /\ (m < n)%nat).
+Proof using. auto. Qed.
+
+Lemma wf_nat_upto : forall (b:nat),
+  wf (nat_upto b).
 Proof using.
   intros b n.
-  induction_wf: (measure_wf (fun n => b-n)) n.
+  induction_wf: (wf_measure (fun n => (b-n)%nat)) n.
   apply Acc_intro. introv [H1 H2]. apply IH.
   hnf. nat_math.
 Qed.
@@ -220,32 +209,29 @@ Qed.
 (** ** The relation "less than" on the set of
        integers greater than a fixed lower bound. *)
 
-Require Import LibInt.
+Definition downto (b:int) :=
+  fun (n m:int) => (b <= n) /\ (n < m).
 
-Definition downto (b : int) :=
-  fun n m : int => (b <= n) /\ (n < m).
-
-(* TODO: rename to downto_eq *)
-
-Lemma downto_def : forall b n m,
+Lemma downto_eq : forall (b n m:int),
   downto b n m = (b <= n /\ n < m).
 Proof using. auto. Qed.
 
-Lemma downto_intro : forall b n m,
+Lemma downto_intro : forall (b n m:int),
   b <= n ->
   n < m -> 
   downto b n m.
 Proof using. split~. Qed.
 
-Lemma downto_wf : forall n, wf (downto n).
+Lemma wf_downto : forall (b:int), 
+  wf (downto b).
 Proof using.
   intros b n.
-  induction_wf: (measure_wf (fun n => Zabs_nat (n-b))) n.
+  induction_wf: (wf_measure (fun n => Zabs_nat (n-b))) n.
   apply Acc_intro. introv [H1 H2]. apply IH.
   unfolds. applys lt_abs_abs; math.
 Qed.
 
-Hint Resolve downto_wf : wf.
+Hint Resolve wf_downto : wf.
 Hint Unfold downto.
 Hint Extern 1 (downto _ _ _) => math : maths.
 
@@ -254,10 +240,10 @@ Hint Extern 1 (downto _ _ _) => math : maths.
 (** ** The relation "greater than" on the set of
        integers lower than a fixed upper bound. *)
 
-Definition upto (b : int) :=
-  fun n m : int => (n <= b) /\ (m < n).
+Definition upto (b:int) :=
+  fun (n m:int) => (n <= b) /\ (m < n).
 
-Lemma upto_def : forall b n m,
+Lemma upto_eq : forall b n m,
   upto b n m = ((n <= b) /\ (m < n)).
 Proof using. auto. Qed.
 
@@ -267,19 +253,18 @@ Lemma upto_intro : forall b n m,
   upto b n m.
 Proof using. split~. Qed.
 
-Lemma upto_wf : forall n, 
+Lemma wf_upto : forall n, 
   wf (upto n).
 Proof using.
   intros b n.
-  induction_wf: (measure_wf (fun n => Zabs_nat (b-n))) n.
+  induction_wf: (wf_measure (fun n => Zabs_nat (b-n))) n.
   apply Acc_intro. introv [H1 H2]. apply IH.
   applys lt_abs_abs; math.
 Qed.
 
-Hint Resolve upto_wf : wf.
+Hint Resolve wf_upto : wf.
 Hint Unfold upto.
 Hint Extern 1 (upto _ _ _) => math : maths.
-
 
 
 (* ********************************************************************** *)
@@ -288,7 +273,7 @@ Hint Extern 1 (upto _ _ _) => math : maths.
 Section UnprojWf.
 Variables (A1 A2 A3 A4 A5 : Type).
 
-Lemma unproj21_wf : forall (R : binary A1),
+Lemma wf_unproj21 : forall (R:binary A1),
   wf R ->
   wf (unproj21 A2 R).
 Proof using.
@@ -296,7 +281,7 @@ Proof using.
   induction_wf IH: H x1. constructor. intros [y1 y2]. auto.
 Qed.
 
-Lemma unproj22_wf : forall (R : binary A2),
+Lemma wf_unproj22 : forall (R:binary A2),
   wf R ->
   wf (unproj22 A1 R).
 Proof using.
@@ -304,7 +289,7 @@ Proof using.
   induction_wf IH: H x2. constructor. intros [y1 y2]. auto.
 Qed.
 
-Lemma unproj31_wf : forall (R : binary A1),
+Lemma wf_unproj31 : forall (R:binary A1),
   wf R ->
   wf (unproj31 A2 A3 R).
 Proof using.
@@ -312,7 +297,7 @@ Proof using.
   induction_wf IH: H x1. constructor. intros [[y1 y2] y3]. auto.
 Qed.
 
-Lemma unproj32_wf : forall (R : binary A2),
+Lemma wf_unproj32 : forall (R:binary A2),
   wf R ->
   wf (unproj32 A1 A3 R).
 Proof using.
@@ -320,7 +305,7 @@ Proof using.
   induction_wf IH: H x2. constructor. intros [[y1 y2] y3]. auto.
 Qed.
 
-Lemma unproj33_wf : forall (R : binary A3),
+Lemma wf_unproj33 : forall (R:binary A3),
   wf R ->
   wf (unproj33 A1 A2 R).
 Proof using.
@@ -328,7 +313,7 @@ Proof using.
   induction_wf IH: H x3. constructor. intros [[y1 y2] y3]. auto.
 Qed.
 
-Lemma unproj41_wf : forall (R : binary A1),
+Lemma wf_unproj41 : forall (R:binary A1),
   wf R ->
   wf (unproj41 A2 A3 A4 R).
 Proof using.
@@ -336,7 +321,7 @@ Proof using.
   induction_wf IH: H x1. constructor. intros [[[y1 y2] y3] y4]. auto.
 Qed.
 
-Lemma unproj42_wf : forall (R : binary A2),
+Lemma wf_unproj42 : forall (R:binary A2),
   wf R ->
   wf (unproj42 A1 A3 A4 R).
 Proof using.
@@ -344,7 +329,7 @@ Proof using.
   induction_wf IH: H x2. constructor. intros [[[y1 y2] y3] y4]. auto.
 Qed.
 
-Lemma unproj43_wf : forall (R : binary A3),
+Lemma wf_unproj43 : forall (R:binary A3),
   wf R ->
   wf (unproj43 A1 A2 A4 R).
 Proof using.
@@ -352,7 +337,7 @@ Proof using.
   induction_wf IH: H x3. constructor. intros [[[y1 y2] y3] y4]. auto.
 Qed.
 
-Lemma unproj44_wf : forall (R : binary A4),
+Lemma wf_unproj44 : forall (R:binary A4),
   wf R ->
   wf (unproj44 A1 A2 A3 R).
 Proof using.
@@ -360,7 +345,7 @@ Proof using.
   induction_wf IH: H x4. constructor. intros [[[y1 y2] y3] y4]. auto.
 Qed.
 
-Lemma unproj51_wf : forall (R : binary A1),
+Lemma wf_unproj51 : forall (R:binary A1),
   wf R ->
   wf (unproj51 A2 A3 A4 A5 R).
 Proof using.
@@ -371,16 +356,16 @@ Qed.
 End UnprojWf.
 
 Hint Resolve
-  unproj21_wf unproj22_wf
-  unproj31_wf unproj32_wf unproj33_wf
-  unproj41_wf unproj42_wf unproj43_wf unproj44_wf
-  unproj51_wf : wf.
+  wf_unproj21 wf_unproj22
+  wf_unproj31 wf_unproj32 wf_unproj33
+  wf_unproj41 wf_unproj42 wf_unproj43 wf_unproj44
+  wf_unproj51 : wf.
 
 
 (* ********************************************************************** *)
 (** * Lexicographical product *)
 
-Lemma lexico2_wf : forall A1 A2
+Lemma wf_lexico2 : forall A1 A2
  (R1:binary A1) (R2:binary A2),
   wf R1 -> 
   wf R2 -> 
@@ -393,17 +378,17 @@ Proof using.
   apply~ IH1. rewrite H1. apply~ IH2.
 Qed.
 
-Lemma lexico3_wf : forall A1 A2 A3
+Lemma wf_lexico3 : forall A1 A2 A3
  (R1:binary A1) (R2:binary A2) (R3:binary A3),
   wf R1 -> 
   wf R2 -> 
   wf R3 ->
   wf (lexico3 R1 R2 R3).
 Proof using.
-  intros. apply~ lexico2_wf. apply~ lexico2_wf.
+  intros. apply~ wf_lexico2. apply~ wf_lexico2.
 Qed.
 
-Lemma lexico4_wf : forall A1 A2 A3 A4
+Lemma wf_lexico4 : forall A1 A2 A3 A4
  (R1:binary A1) (R2:binary A2) (R3:binary A3) (R4:binary A4),
   wf R1 -> 
   wf R2 -> 
@@ -411,26 +396,26 @@ Lemma lexico4_wf : forall A1 A2 A3 A4
   wf R4 ->
   wf (lexico4 R1 R2 R3 R4).
 Proof using.
-  intros. apply~ lexico3_wf. apply~ lexico2_wf.
+  intros. apply~ wf_lexico3. apply~ wf_lexico2.
 Qed.
 
-Hint Resolve lexico2_wf lexico3_wf lexico4_wf : wf.
-
+Hint Resolve wf_lexico2 wf_lexico3 wf_lexico4 : wf.
 
 
 (* ********************************************************************** *)
 (** * Symmetric product *)
 
-Lemma prod2_wf_1 : forall (A1 A2:Type)
+Lemma wf_prod2_of_wf_1 : forall (A1 A2:Type)
  (R1:binary A1) (R2:binary A2),
-  wf R1 -> wf (prod2 R1 R2).
+  wf R1 -> 
+  wf (prod2 R1 R2).
 Proof using.
   introv W1. intros [x1 x2].
   gen x2. induction_wf IH: W1 x1. intros.
   constructor. intros [y1 y2] [E1 E2]. apply~ IH.
 Qed.
 
-Lemma prod2_wf_2 : forall (A1 A2:Type)
+Lemma wf_prod2_of_wf_2 : forall (A1 A2:Type)
  (R1:binary A1) (R2:binary A2),
   wf R2 -> 
   wf (prod2 R1 R2).
@@ -440,89 +425,73 @@ Proof using.
   constructor. intros [y1 y2] [E1 E2]. apply~ IH.
 Qed.
 
-Lemma prod3_wf_1 : forall (A1 A2 A3:Type)
+Lemma wf_prod3_of_wf_1 : forall (A1 A2 A3:Type)
  (R1:binary A1) (R2:binary A2) (R3:binary A3),
   wf R1 -> 
   wf (prod3 R1 R2 R3).
-Proof using. intros. apply prod2_wf_1. apply~ prod2_wf_1. Qed.
+Proof using. intros. apply wf_prod2_of_wf_1. apply~ wf_prod2_of_wf_1. Qed.
 
-Lemma prod3_wf_2 : forall (A1 A2 A3:Type)
+Lemma wf_prod3_of_wf_2 : forall (A1 A2 A3:Type)
  (R1:binary A1) (R2:binary A2) (R3:binary A3),
   wf R2 -> 
   wf (prod3 R1 R2 R3).
-Proof using. intros. apply prod2_wf_1. apply~ prod2_wf_2. Qed.
+Proof using. intros. apply wf_prod2_of_wf_1. apply~ wf_prod2_of_wf_2. Qed.
 
-Lemma prod3_wf_3 : forall (A1 A2 A3:Type)
+Lemma wf_prod3_of_wf_3 : forall (A1 A2 A3:Type)
  (R1:binary A1) (R2:binary A2) (R3:binary A3),
   wf R3 -> 
   wf (prod3 R1 R2 R3).
-Proof using. intros. apply~ prod2_wf_2. Qed.
+Proof using. intros. apply~ wf_prod2_of_wf_2. Qed.
 
-Lemma prod4_wf_1 : forall (A1 A2 A3 A4:Type)
+Lemma wf_prod4_of_wf_1 : forall (A1 A2 A3 A4:Type)
  (R1:binary A1) (R2:binary A2) (R3:binary A3) (R4:binary A4),
   wf R1 -> 
   wf (prod4 R1 R2 R3 R4).
-Proof using. intros. apply prod2_wf_1. apply~ prod3_wf_1. Qed.
+Proof using. intros. apply wf_prod2_of_wf_1. apply~ wf_prod3_of_wf_1. Qed.
 
-Lemma prod4_wf_2 : forall (A1 A2 A3 A4:Type)
+Lemma wf_prod4_of_wf_2 : forall (A1 A2 A3 A4:Type)
  (R1:binary A1) (R2:binary A2) (R3:binary A3) (R4:binary A4),
   wf R2 -> 
   wf (prod4 R1 R2 R3 R4).
-Proof using. intros. apply prod2_wf_1. apply~ prod3_wf_2. Qed.
+Proof using. intros. apply wf_prod2_of_wf_1. apply~ wf_prod3_of_wf_2. Qed.
 
-Lemma prod4_wf_3 : forall (A1 A2 A3 A4:Type)
+Lemma wf_prod4_of_wf_3 : forall (A1 A2 A3 A4:Type)
  (R1:binary A1) (R2:binary A2) (R3:binary A3) (R4:binary A4),
   wf R3 -> 
   wf (prod4 R1 R2 R3 R4).
-Proof using. intros. apply prod2_wf_1. apply~ prod3_wf_3. Qed.
+Proof using. intros. apply wf_prod2_of_wf_1. apply~ wf_prod3_of_wf_3. Qed.
 
-Lemma prod4_wf_4 : forall (A1 A2 A3 A4:Type)
+Lemma wf_prod4_of_wf_4 : forall (A1 A2 A3 A4:Type)
  (R1:binary A1) (R2:binary A2) (R3:binary A3) (R4:binary A4),
   wf R4 -> 
   wf (prod4 R1 R2 R3 R4).
-Proof using. intros. apply~ prod2_wf_2. Qed.
+Proof using. intros. apply~ wf_prod2_of_wf_2. Qed.
 
 Hint Resolve
-  prod2_wf_1 prod2_wf_2
-  prod3_wf_1 prod3_wf_2 prod3_wf_3
-  prod4_wf_1 prod4_wf_2 prod4_wf_3 prod4_wf_4 : wf.
+  wf_prod2_of_wf_1 wf_prod2_of_wf_2
+  wf_prod3_of_wf_1 wf_prod3_of_wf_2 wf_prod3_of_wf_3
+  wf_prod4_of_wf_1 wf_prod4_of_wf_2 wf_prod4_of_wf_3 wf_prod4_of_wf_4 : wf.
 
 
 (* ********************************************************************** *)
 (** * Well-foundedness of a function image *)
 
-Definition binary_map A B (f:A->B) (R:binary B) : binary A :=
-  fun x y => R (f x) (f y).
-
-Lemma binary_map_wf : forall A B (f:A->B) (R:binary B),
-  wf R -> wf (binary_map f R).
+Lemma wf_rel_preimage : forall A B (R:binary B) (f:A->B),
+  wf R -> 
+  wf (rel_preimage R f).
 Proof using.
   introv W. intros x. gen_eq a: (f x). gen x.
   induction_wf: W a. introv E. constructors.
   intros y Hy. subst a. hnf in Hy. applys* IH.
 Qed.
 
-Hint Resolve binary_map_wf : wf.
+Hint Resolve wf_rel_preimage : wf.
 
 
 (* ********************************************************************** *)
-(** * Inverse image *)
-
-Lemma inverse_image_wf : forall (A B : Type) (R : binary B) (f : A -> B),
-  wf R -> 
-  wf (inverse_image R f).
-Proof using.
-  introv W. intros x. gen_eq y: (f x). gen x.
-  induction_wf IH: W y. intros u E. subst y.
-  constructor. intros v I. applys~ IH (f v).
-Qed.
-
-Hint Resolve inverse_image_wf : wf.
-
-(* todo: inverse image of relation ? *)
-
-
-
+(* ********************************************************************** *)
+(* ********************************************************************** *)
+(* TEMPORARY *)
 
 (* begin hide *)
 
